verified/secprop/integ_ni.i.dfy
@@ -1,0 +1,83 @@
+include "sec_prop.s.dfy"
+include "../pagedb.s.dfy"
+include "../entry.s.dfy"
+include "sec_prop_util.i.dfy"
+include "enc_ni_entry.i.dfy"
+include "conf_ni.i.dfy"
+
+//-----------------------------------------------------------------------------
+// NI proof of integriy
+//-----------------------------------------------------------------------------
+// The integrity of an observer enclave, obs, is protected from a malicious
+// OS colluding with an enclave.
+lemma lemma_enc_ni(s1: state, d1: PageDb, s1': state, d1': PageDb,
+                   s2: state, d2: PageDb, s2': state, d2': PageDb,
+                   obs: PageNr)
+    requires ni_reqs(s1, d1, s1', d1', s2, d2, s2', d2', obs)
+    requires smchandler(s1, d1, s1', d1')
+    requires smchandler(s2, d2, s2', d2')
+    requires same_call_args(s1, s2)
+    requires InsecureMemInvariant(s1, s2) // public input to mapSecure.
+    requires loweq_pdb(d1, d2, obs)
+    requires s1.conf.nondet == s2.conf.nondet
+    ensures loweq_pdb(d1', d2', obs)
+    // ensures !(var callno := s1.regs[R0]; var asp := s1.regs[R1];
+    //     callno == KOM_SMC_STOP && asp == obs) ==>
+    //     loweq_pdb(d1', d2', obs)
+{
+    reveal ValidRegState();
+    var callno, arg1, arg2, arg3, arg4
+        := s1.regs[R0], s1.regs[R1], s1.regs[R2], s1.regs[R3], s1.regs[R4];
+    var e1', e2' := s1'.regs[R0], s2'.regs[R0];
+
+    if(callno == KOM_SMC_QUERY || callno == KOM_SMC_GETPHYSPAGES){
+        assert d1' == d1;
+        assert d2' == d2;
+        reveal loweq_pdb();
+    }
+    else if(callno == KOM_SMC_INIT_ADDRSPACE){
+        lemma_initAddrspace_loweq_pdb(d1, d1', e1', d2, d2', e2', arg1, arg2, obs);
+    }
+    else if(callno == KOM_SMC_INIT_DISPATCHER){
+        lemma_initDispatcher_loweq_pdb(d1, d1', e1', d2, d2', e2', arg1, arg2, arg3, obs);
+    }
+    else if(callno == KOM_SMC_INIT_L2PTABLE){
+        lemma_initL2PTable_loweq_pdb(d1, d1', e1', d2, d2', e2', arg1, arg2, arg3, obs);
+    }
+    else if(callno == KOM_SMC_MAP_SECURE){
+        assert loweq_pdb(d1', d2', obs) by {
+            reveal loweq_pdb();
+            var c1 := maybeContentsOfPhysPage(s1, arg4);
+            var c2 := maybeContentsOfPhysPage(s2, arg4);
+            assert contentsOk(arg4, c1) && contentsOk(arg4, c2);
+            lemma_maybeContents_insec_ni(s1, s2, c1, c2, arg4);
+            assert c1 == c2;
+            lemma_mapSecure_loweq_pdb(d1, d1', e1', c1, d2, d2', e2', c2,
+                arg1, arg2, arg3, arg4, obs);
+        }
+    }
+    else if(callno == KOM_SMC_ALLOC_SPARE) {
+        lemma_allocSpare_loweq_pdb(d1, d1', e1', d2, d2', e2', arg1, arg2, obs);
+    }
+    else if(callno == KOM_SMC_MAP_INSECURE){
+        lemma_mapInsecure_loweq_pdb(d1, d1', e1', d2, d2', e2', arg1, arg2, arg3, obs);
+    }
+    else if(callno == KOM_SMC_REMOVE){
+        lemma_remove_loweq_pdb(d1, d1', e1', d2, d2', e2', arg1, obs);
+    }
+    else if(callno == KOM_SMC_FINALISE){
+        lemma_finalise_loweq_pdb(d1, d1', e1', d2, d2', e2', arg1, obs);
+    }
+    else if(callno == KOM_SMC_ENTER){
+        lemma_enter_enc_ni(s1, d1, s1', d1', s2, d2, s2', d2', arg1, arg2, arg3, arg4, obs);
+    }
+    else if(callno == KOM_SMC_RESUME){
+        lemma_resume_enc_ni(s1, d1, s1', d1', s2, d2, s2', d2', arg1, obs);
+    }
+    else if(callno == KOM_SMC_STOP){
+        lemma_stop_loweq_pdb(d1, d1', e1', d2, d2', e2', arg1, obs);
+    }
+    else {
+        reveal loweq_pdb();
+    }
+}
