verified/secprop/integ_ni_entry.i.dfy
@@ -1,0 +1,851 @@
+include "sec_prop.s.dfy"
+include "../pagedb.s.dfy"
+include "../entry.s.dfy"
+include "sec_prop_util.i.dfy"
+include "../smcapi.i.dfy"
+include "conf_ni_entry.i.dfy"
+
+lemma lemma_enter_enc_ni(s1: state, d1: PageDb, s1':state, d1': PageDb,
+                              s2: state, d2: PageDb, s2':state, d2': PageDb,
+                              dispPage: word, arg1: word, arg2: word, arg3: word,
+                              obs: PageNr)
+    requires ni_reqs(s1, d1, s1', d1', s2, d2, s2', d2', obs)
+    requires smc_enter(s1, d1, s1', d1', dispPage, arg1, arg2, arg3)
+    requires smc_enter(s2, d2, s2', d2', dispPage, arg1, arg2, arg3)
+    requires loweq_pdb(d1, d2, obs)
+    requires s1.conf.nondet == s2.conf.nondet
+    ensures loweq_pdb(d1', d2', obs)
+{
+    reveal loweq_pdb();
+    var e1, e2 := smc_enter_err(d1, dispPage, false), smc_enter_err(d2, dispPage, false);
+
+    assert e1 == KOM_ERR_SUCCESS <==> e2 == KOM_ERR_SUCCESS;
+
+    if(e1 == KOM_ERR_SUCCESS && e2 == KOM_ERR_SUCCESS) {
+        var asp1, asp2 := d1[dispPage].addrspace, d2[dispPage].addrspace;
+        assert asp1 == asp2;
+        if(asp1 == obs) {
+            lemma_enter_enc_obs_enter(s1, d1, s1', d1',
+                                       s2, d2, s2', d2',
+                                       dispPage, arg1, arg2, arg3, 
+                                       obs, false);
+        } else {
+            lemma_enter_loweq_pdb_not_obs(s1, d1, s1', d1',
+                                           s2, d2, s2', d2',
+                                           dispPage, arg1, arg2, arg3,
+                                           asp1, obs, false);
+        }
+    }
+    if(e1 != KOM_ERR_SUCCESS && e2 != KOM_ERR_SUCCESS) {
+        assert loweq_pdb(d1', d2', obs);
+    }
+
+}
+
+lemma
+lemma_enter_loweq_pdb_not_obs(s1: state, d1: PageDb, s1':state, d1': PageDb,
+                               s2: state, d2: PageDb, s2':state, d2': PageDb,
+                               dispPage: word, arg1: word, arg2: word, arg3: word,
+                               asp: PageNr,obs: PageNr, isresume:bool)
+    requires ni_reqs(s1, d1, s1', d1', s2, d2, s2', d2', obs)
+    requires valAddrPage(d1, asp) && valAddrPage(d2, asp)
+    requires !isresume ==> smc_enter(s1, d1, s1', d1', dispPage, arg1, arg2, arg3)
+    requires !isresume ==> smc_enter(s2, d2, s2', d2', dispPage, arg1, arg2, arg3)
+    requires isresume ==> smc_resume(s1, d1, s1', d1', dispPage)
+    requires isresume ==> smc_resume(s2, d2, s2', d2', dispPage)
+    requires validPageNr(dispPage) && d1[dispPage].PageDbEntryTyped? && 
+        d2[dispPage].PageDbEntryTyped?
+    requires d1[dispPage].addrspace == asp && d2[dispPage].addrspace == asp
+    requires asp != obs
+    requires loweq_pdb(d1, d2, obs)
+    requires smc_enter_err(d1, dispPage, isresume) == KOM_ERR_SUCCESS
+            && (smc_enter_err(d2, dispPage, isresume) == KOM_ERR_SUCCESS);
+    requires s1.conf.nondet == s2.conf.nondet
+    ensures  loweq_pdb(d1', d2', obs)
+{
+    if(!isresume) {
+        var s11:state, steps1: nat :|
+            preEntryEnter(s1, s11, d1, dispPage, arg1, arg2, arg3) &&
+            validEnclaveExecution(s11, d1, s1', d1', dispPage, steps1);
+        
+        var s21:state, steps2: nat :|
+            preEntryEnter(s2, s21, d2, dispPage, arg1, arg2, arg3) &&
+            validEnclaveExecution(s21, d2, s2', d2', dispPage, steps2);
+
+        assert s11.conf.nondet == s21.conf.nondet;
+        assert user_regs(s11.regs) == user_regs(s21.regs);
+
+        assert !spsr_of_state(s11).f && !spsr_of_state(s11).i &&
+            !spsr_of_state(s21).f && !spsr_of_state(s21).i by {
+            assert psr_mask_fiq(encode_mode(User)) == 0 by {
+                assert WordAsBits(0x10) == 0x10 && WordAsBits(0x40) == 0x40
+                    by { reveal WordAsBits(); }
+                lemma_BitsAndWordConversions();
+                reveal BitAnd();
+            }
+            assert psr_mask_irq(encode_mode(User)) == 0 by {
+                assert WordAsBits(0x10) == 0x10 && WordAsBits(0x80) == 0x80
+                    by { reveal WordAsBits(); }
+                lemma_BitsAndWordConversions();
+                reveal BitAnd();
+            }
+        }
+        lemma_validEnclaveEx_enc_not_obs(s11, d1, s1', d1', s21, d2, s2', d2',
+                                         dispPage, steps1, steps2, asp, obs);
+    } else {
+        var s11:state, steps1: nat :|
+            preEntryResume(s1, s11, d1, dispPage) &&
+            validEnclaveExecution(s11, d1, s1', d1', dispPage, steps1);
+        
+        var s21:state, steps2: nat :|
+            preEntryResume(s2, s21, d2, dispPage) &&
+            validEnclaveExecution(s21, d2, s2', d2', dispPage, steps2);
+
+        assert s11.conf.nondet == s21.conf.nondet;
+
+        lemma_validEnclaveEx_enc_not_obs(s11, d1, s1', d1', s21, d2, s2', d2',
+                                     dispPage, steps1, steps2, asp, obs);
+    }
+}
+
+lemma lemma_validEnclaveEx_enc_not_obs(s1: state, d1: PageDb, s1':state, d1': PageDb,
+                                        s2: state, d2: PageDb, s2':state, d2': PageDb,
+                                        dispPg: PageNr, steps1:nat, steps2:nat,
+                                        asp: PageNr, obs: PageNr)
+    
+    requires ValidState(s1) && ValidState(s2) &&
+             ValidState(s1') && ValidState(s2') &&
+             validPageDb(d1) && validPageDb(d2) && 
+             validPageDb(d1') && validPageDb(d2') && SaneConstants()
+    requires do_declassify()
+    requires valAddrPage(d1, asp) && valAddrPage(d2, asp)
+    requires valAddrPage(d1, obs) && valAddrPage(d2, obs)
+    requires finalDispatcher(d1, dispPg) && finalDispatcher(d2, dispPg)
+    requires d1[dispPg].addrspace == asp && d2[dispPg].addrspace == asp
+    requires asp != obs
+    requires validEnclaveExecution(s1, d1, s1', d1', dispPg, steps1)
+    requires validEnclaveExecution(s2, d2, s2', d2', dispPg, steps2);
+    requires loweq_pdb(d1, d2, obs)
+    requires s1.conf.nondet == s2.conf.nondet
+    requires mode_of_state(s1) != User && mode_of_state(s2) != User
+    requires !spsr_of_state(s1).f && !spsr_of_state(s1).i
+    requires !spsr_of_state(s2).f && !spsr_of_state(s2).i
+    requires s1.conf.scr == s2.conf.scr;
+    // requires InsecureMemInvariant(s1, s2)
+    ensures  loweq_pdb(d1', d2', obs)
+    ensures  same_ret(s1', s2')
+    ensures  valAddrPage(d1', asp) && valAddrPage(d2', asp)
+    ensures  valAddrPage(d1', obs) && valAddrPage(d2', obs)
+    ensures finalDispatcher(d1', dispPg) && finalDispatcher(d2', dispPg)
+    ensures  d1'[dispPg].addrspace == asp && d2'[dispPg].addrspace == asp
+    // ensures InsecureMemInvariant(s1', s2')
+    decreases steps1, steps2
+{
+    reveal validEnclaveExecution();
+
+    var retToEnclave1, s15, d15 := lemma_unpack_validEnclaveExecution(
+        s1, d1, s1', d1', dispPg, steps1);
+    var retToEnclave2, s25, d25 := lemma_unpack_validEnclaveExecution(
+        s2, d2, s2', d2', dispPg, steps2);
+
+    lemma_validEnclaveExecutionStep_validPageDb(s1, d1, s15, d15, dispPg, retToEnclave1);
+    lemma_validEnclaveExecutionStep_validPageDb(s2, d2, s25, d25, dispPg, retToEnclave2);
+    lemma_validEnclaveStep_enc_not_obs(s1, d1, s15, d15, s2, d2, s25, d25,
+        dispPg, retToEnclave1, retToEnclave2, asp, obs);
+
+    assert retToEnclave1 == retToEnclave2;
+
+    if(retToEnclave1) {
+        lemma_validEnclaveExecution(s15, d15, s1', d1', dispPg, steps1 - 1);
+        lemma_validEnclaveExecution(s25, d25, s2', d2', dispPg, steps2 - 1);
+        lemma_validEnclaveEx_enc_not_obs(s15, d15, s1', d1', s25, d25, s2', d2',
+                                         dispPg, steps1 - 1, steps2 - 1, asp, 
+                                         obs);
+    } else {
+        reveal loweq_pdb();
+    }
+}
+
+lemma lemma_validEnclaveStep_enc_not_obs(s1: state, d1: PageDb, s1':state, d1': PageDb,
+                                          s2: state, d2: PageDb, s2':state, d2': PageDb,
+                                          dispPg: PageNr, ret1:bool, ret2:bool,
+                                          asp: PageNr, obs: PageNr)
+    requires ValidState(s1) && ValidState(s2) &&
+             ValidState(s1') && ValidState(s2') &&
+             validPageDb(d1) && validPageDb(d2) && 
+             validPageDb(d1') && validPageDb(d2') && SaneConstants()
+    requires do_declassify()
+    requires valAddrPage(d1, asp) && valAddrPage(d2, asp)
+    requires valAddrPage(d1, obs) && valAddrPage(d2, obs)
+    requires finalDispatcher(d1, dispPg)
+    requires finalDispatcher(d2, dispPg)
+    requires d1[dispPg].addrspace == asp && d2[dispPg].addrspace == asp
+    requires asp != obs
+    // requires InsecureMemInvariant(s1, s2)
+    requires validEnclaveExecutionStep(s1, d1, s1', d1', dispPg, ret1);
+    requires validEnclaveExecutionStep(s2, d2, s2', d2', dispPg, ret2);
+    requires loweq_pdb(d1, d2, obs)
+    requires s1.conf.nondet == s2.conf.nondet
+    requires mode_of_state(s1) != User && mode_of_state(s2) != User
+    requires !spsr_of_state(s1).f && !spsr_of_state(s1).i
+    requires !spsr_of_state(s2).f && !spsr_of_state(s2).i
+    requires s1.conf.scr == s2.conf.scr;
+    ensures  loweq_pdb(d1', d2', obs)
+    ensures  ret1 == ret2
+    ensures  ret1 ==> s1'.conf.nondet == s2'.conf.nondet;
+    ensures  !ret1 ==> same_ret(s1', s2')
+    ensures  valAddrPage(d1', asp)  && valAddrPage(d2', asp)
+    ensures  valAddrPage(d1', obs) && valAddrPage(d2', obs)
+    ensures finalDispatcher(d1', dispPg) && finalDispatcher(d2', dispPg)
+    ensures  d1'[dispPg].addrspace == asp && d2'[dispPg].addrspace == asp
+    // ensures  InsecureMemInvariant(s1', s2')
+{
+    reveal validEnclaveExecutionStep();
+    var s14, d14 :|
+        validEnclaveExecutionStep'(s1, d1, s14, d14, s1', d1',
+            dispPg, ret1);
+
+    var s24, d24 :|
+        validEnclaveExecutionStep'(s2, d2, s24, d24, s2', d2',
+            dispPg, ret2);
+
+    lemma_validEnclaveStepPrime_enc_not_obs(
+        s1, d1, s14, d14, s1', d1',
+        s2, d2, s24, d24, s2', d2',
+        dispPg, ret1, ret2, asp, obs);
+}
+
+lemma {:timeLimitMultiplier 3}
+lemma_validEnclaveStepPrime_enc_not_obs(
+s11: state, d11: PageDb, s14:state, d14:PageDb, r1:state, rd1:PageDb,
+s21: state, d21: PageDb, s24:state, d24:PageDb, r2:state, rd2:PageDb,
+dispPg:PageNr, retToEnclave1:bool, retToEnclave2:bool,
+asp: PageNr, obs: PageNr)
+    requires ValidState(s11) && ValidState(s21) &&
+             ValidState(r1)  && ValidState(r2)  &&
+             validPageDb(d11) &&
+             validPageDb(d21) && 
+             validPageDb(d14) && 
+             validPageDb(d24) && 
+             validPageDb(rd1) && 
+             validPageDb(rd2) && 
+             SaneConstants()
+    requires do_declassify()
+    requires valAddrPage(d11, asp) && valAddrPage(d21, asp)
+    requires valAddrPage(d11, obs) && valAddrPage(d21, obs)
+    requires finalDispatcher(d11, dispPg)
+    requires finalDispatcher(d21, dispPg)
+    requires validEnclaveExecutionStep'(s11,d11,s14,d14,r1,rd1,dispPg,retToEnclave1)
+    requires validEnclaveExecutionStep'(s21,d21,s24,d24,r2,rd2,dispPg,retToEnclave2)
+    // requires InsecureMemInvariant(s11, s21)
+    requires d11[dispPg].addrspace == asp && d21[dispPg].addrspace == asp
+    requires asp != obs
+    requires loweq_pdb(d11, d21, obs)
+    requires s11.conf.nondet == s21.conf.nondet
+    requires mode_of_state(s11) != User && mode_of_state(s21) != User
+    // requires spsr_same(s11, s21)
+    requires s11.conf.scr == s21.conf.scr;
+    ensures  loweq_pdb(rd1, rd2, obs)
+    // ensures  InsecureMemInvariant(r1, r2)
+    ensures  retToEnclave1 == retToEnclave2
+    ensures  retToEnclave1 ==> r1.conf.scr == r2.conf.scr
+    ensures  retToEnclave1 ==> r1.conf.nondet == r2.conf.nondet
+    ensures  !retToEnclave1 ==> same_ret(r1, r2)
+    ensures  valAddrPage(rd1, asp)  && valAddrPage(rd2, asp)
+    ensures  valAddrPage(rd1, obs) && valAddrPage(rd2, obs)
+    ensures finalDispatcher(rd1, dispPg) && finalDispatcher(rd2, dispPg)
+    ensures  rd1[dispPg].addrspace == asp && rd2[dispPg].addrspace == asp
+    // ensures  retToEnclave1 ==> OperandContents(r1, OLR) == OperandContents(r2, OLR)
+    // ensures  retToEnclave1 ==> user_regs(r1.regs) == user_regs(r2.regs)
+{    
+    assert l1pOfDispatcher(d11, dispPg) == l1pOfDispatcher(d21, dispPg) by
+        { reveal loweq_pdb(); }
+    var l1p := l1pOfDispatcher(d11, dispPg);
+
+    assert dataPagesCorrespond(s11.m, d11);
+    assert dataPagesCorrespond(s21.m, d21);
+    
+    assert userspaceExecutionAndException(s11, s14);
+    assert userspaceExecutionAndException(s21, s24);
+    
+    reveal userspaceExecutionAndException();
+
+    var s1', s12 :| userspaceExecutionAndException'(s11, s1', s12, s14);
+    var s2', s22 :| userspaceExecutionAndException'(s21, s2', s22, s24);
+
+    var pc1 := OperandContents(s11, OLR);
+    var pc2 := OperandContents(s21, OLR);
+    
+    assert ExtractAbsPageTable(s12).Just? by {
+        assert ExtractAbsPageTable(s11).Just?;
+        assert ExtractAbsPageTable(s11) == ExtractAbsPageTable(s1');
+        assert ExtractAbsPageTable(s12) == ExtractAbsPageTable(s1');
+    }
+    var (s13, expc1, ex1) := userspaceExecutionFn(s12, pc1);
+    var (s23, expc2, ex2) := userspaceExecutionFn(s22, pc2);
+  
+    /*
+    assert InsecureMemInvariant(s12, s22) by {
+        assert InsecureMemInvariant(s11, s12);
+        assert InsecureMemInvariant(s21, s22);
+    }
+    */
+
+    var pt1 := ExtractAbsPageTable(s12);
+    var pt2 := ExtractAbsPageTable(s22);
+
+    assert pageTableCorresponds(s12, d11, l1p)
+        && pageTableCorresponds(s22, d21, l1p) by
+    { 
+        assert pageTableCorresponds(s11, d11, l1p);
+        assert pageTableCorresponds(s21, d21, l1p);
+        reveal pageTableCorresponds();
+    }
+
+    assert pt1 == pt2 by {
+        lemma_eqpdb_pt_coresp_not_atkr(d11, d21, s12, s22, l1p, asp, obs);
+    }
+
+    assert s12.conf.nondet == s22.conf.nondet;
+
+    /*
+    assert InsecureMemInvariant(s13, s23) by {
+        lemma_insecure_mem_userspace(
+            s12, pc1, s13, expc1, ex1,
+            s22, pc2, s23, expc2, ex2);
+    }
+
+    assert InsecureMemInvariant(s14, s24);
+
+    assert InsecureMemInvariant(r1, r2);
+    */
+
+    assert s13.conf.nondet == s23.conf.nondet by
+    {
+        reveal userspaceExecutionFn();
+        assert s13.conf.nondet == nondet_int(s12.conf.nondet, NONDET_GENERATOR());
+        assert s23.conf.nondet == nondet_int(s22.conf.nondet, NONDET_GENERATOR());
+    }
+    
+    assert s14.conf.nondet == s24.conf.nondet;
+
+    assert ex1 == ex2 && s14.conf.ex == s24.conf.ex by {
+        lemma_decl_ex(s1', s12, s14, s2', s22, s24);
+    }
+
+    assert loweq_pdb(d14, d24, obs) by
+    {
+        assert validPageDbs({d11,d21,d14,d24});
+        lemma_updateUserPages_conf_not_atkr(s14, d11, d14,
+            s24, d21, d24, dispPg, asp, obs);
+    }
+
+    assert valAddrPage(d14, obs) && valAddrPage(d24, obs) &&
+        d14[dispPg].addrspace == asp && d24[dispPg].addrspace == asp by
+        { reveal updateUserPagesFromState(); }
+
+    assert retToEnclave1 == retToEnclave2 &&
+        (ex1 == ExSVC ==> s14.regs[R0] == s24.regs[R0]) &&
+        (ex1 == ExSVC && (s14.regs[R0] == KOM_SVC_EXIT ||
+            s14.regs[R0] == KOM_SVC_MAP_DATA ||
+            s14.regs[R0] == KOM_SVC_UNMAP_DATA ||
+            s14.regs[R0] == KOM_SVC_INIT_L2PTABLE) ==>
+            s14.regs[R1] == s24.regs[R1]) &&
+        (ex1 == ExSVC && (s14.regs[R0] == KOM_SVC_MAP_DATA ||
+            s14.regs[R0] == KOM_SVC_UNMAP_DATA ||
+            s14.regs[R0] == KOM_SVC_INIT_L2PTABLE) ==>
+            s14.regs[R2] == s24.regs[R2]) by
+    {
+        assert s14.regs[R0] == s13.regs[R0];
+        assert s24.regs[R0] == s23.regs[R0];
+        reveal userspaceExecutionFn();
+        if(ex1 == ExSVC) {
+            lemma_decl_svc_r0(s13, s14, s23, s24);
+            if(s14.regs[R0] == KOM_SVC_EXIT ||
+               s14.regs[R0] == KOM_SVC_MAP_DATA ||
+               s14.regs[R0] == KOM_SVC_UNMAP_DATA ||
+               s14.regs[R0] == KOM_SVC_INIT_L2PTABLE){
+                lemma_decl_svc_r1(s13, s14, s23, s24);
+            }
+            if(s14.regs[R0] == KOM_SVC_MAP_DATA ||
+               s14.regs[R0] == KOM_SVC_UNMAP_DATA ||
+               s14.regs[R0] == KOM_SVC_INIT_L2PTABLE){
+                lemma_decl_svc_r2(s13, s14, s23, s24);
+            }
+        }
+    }
+   
+    lemma_validEnclaveStepPrime_conf_not_atkr_retnondet(
+        s11, d11, s14, d14, r1, rd1,
+        s21, d21, s24, d24, r2, rd2,
+        dispPg, retToEnclave1, retToEnclave2, asp, obs);
+
+}
+
+lemma lemma_enter_enc_obs_enter(s1: state, d1: PageDb, s1':state, d1': PageDb,
+                                 s2: state, d2: PageDb, s2':state, d2': PageDb,
+                                 dispPg: word, arg1: word, arg2: word, arg3: word,
+                                 obs: PageNr, isresume:bool)
+    requires ni_reqs(s1, d1, s1', d1', s2, d2, s2', d2', obs)
+    requires !isresume ==> smc_enter(s1, d1, s1', d1', dispPg, arg1, arg2, arg3)
+    requires !isresume ==> smc_enter(s2, d2, s2', d2', dispPg, arg1, arg2, arg3)
+    requires isresume ==> smc_resume(s1, d1, s1', d1', dispPg)
+    requires isresume ==> smc_resume(s2, d2, s2', d2', dispPg)
+    requires loweq_pdb(d1, d2, obs)
+    requires entering_obs(d1, d2, dispPg, obs, isresume);
+    requires s1.conf.nondet == s2.conf.nondet
+    ensures  loweq_pdb(d1', d2', obs)
+{
+
+    if(!isresume) {
+        var s11:state, steps1: nat :|
+            preEntryEnter(s1, s11, d1, dispPg, arg1, arg2, arg3) &&
+            validEnclaveExecution(s11, d1, s1', d1', dispPg, steps1);
+        
+        var s21:state, steps2: nat :|
+            preEntryEnter(s2, s21, d2, dispPg, arg1, arg2, arg3) &&
+            validEnclaveExecution(s21, d2, s2', d2', dispPg, steps2);
+
+        assert s11.conf.nondet == s21.conf.nondet;
+        assert user_regs(s11.regs) == user_regs(s21.regs);
+
+        assert OperandContents(s11, OLR) == OperandContents(s21, OLR) by 
+        {
+            assert OperandContents(s11, OLR) == d1[dispPg].entry.entrypoint;
+            assert OperandContents(s21, OLR) == d2[dispPg].entry.entrypoint;
+            reveal loweq_pdb();
+        }
+        
+        assert spsr_same(s11, s21) by {
+            assert preEntryEnter(s1, s11, d1, dispPg, arg1, arg2, arg3);
+            assert preEntryEnter(s2, s21, d2, dispPg, arg1, arg2, arg3);
+            var mode1 := mode_of_state(s11);
+            var mode2 := mode_of_state(s21);
+            assert mode1 != User && mode2 != User;
+            reveal ValidSRegState();
+            assert s11.sregs[spsr(mode1)] == encode_mode(User);
+            assert s21.sregs[spsr(mode2)] == encode_mode(User);
+        }
+
+        assert !spsr_of_state(s11).f && !spsr_of_state(s11).i &&
+            !spsr_of_state(s21).f && !spsr_of_state(s21).i by {
+            assert psr_mask_fiq(encode_mode(User)) == 0 by {
+                assert WordAsBits(0x10) == 0x10 && WordAsBits(0x40) == 0x40
+                    by { reveal WordAsBits(); }
+                lemma_BitsAndWordConversions();
+                reveal BitAnd();
+            }
+            assert psr_mask_irq(encode_mode(User)) == 0 by {
+                assert WordAsBits(0x10) == 0x10 && WordAsBits(0x80) == 0x80
+                    by { reveal WordAsBits(); }
+                lemma_BitsAndWordConversions();
+                reveal BitAnd();
+            }
+        }
+        lemma_validEnclaveEx_enc(s11, d1, s1', d1', s21, d2, s2', d2',
+                                             dispPg, steps1, steps2, obs);
+    } else {
+        var s11:state, steps1: nat :|
+            preEntryResume(s1, s11, d1, dispPg) &&
+            validEnclaveExecution(s11, d1, s1', d1', dispPg, steps1);
+        
+        var s21:state, steps2: nat :|
+            preEntryResume(s2, s21, d2, dispPg) &&
+            validEnclaveExecution(s21, d2, s2', d2', dispPg, steps2);
+
+        assert s11.conf.nondet == s21.conf.nondet;
+
+        assert d1[dispPg].entry == d2[dispPg].entry by
+            { reveal loweq_pdb(); }
+
+        assert user_regs(s11.regs) == user_regs(s21.regs) by {
+            var disp := d1[dispPg].entry;
+            assert (forall r | r in USER_REGS() :: 
+                (s11.regs[r] == disp.ctxt.regs[r] &&
+                 s21.regs[r] == disp.ctxt.regs[r]));
+            eqregs(user_regs(s11.regs), user_regs(s21.regs));
+        }
+
+        assert OperandContents(s11, OLR) == OperandContents(s21, OLR) by 
+        {   
+            assert OperandContents(s11, OLR) == d1[dispPg].entry.ctxt.pc;
+            assert OperandContents(s21, OLR) == d2[dispPg].entry.ctxt.pc;
+            reveal loweq_pdb();
+        }
+        
+        assert spsr_same(s11, s21) by {
+            var disp := d1[dispPg].entry;
+            assert preEntryResume(s1, s11, d1, dispPg);
+            assert preEntryResume(s2, s21, d2, dispPg);
+            reveal ValidSRegState();
+            var mode1 := mode_of_state(s11);
+            var mode2 := mode_of_state(s21);
+            assert mode1 != User && mode2 != User;
+            assert s11.sregs[spsr(mode1)] == disp.ctxt.cpsr;
+            assert s21.sregs[spsr(mode2)] == disp.ctxt.cpsr;
+        }
+        lemma_validEnclaveEx_enc(s11, d1, s1', d1', s21, d2, s2', d2',
+                                             dispPg, steps1, steps2, obs);
+    }
+}
+
+lemma lemma_validEnclaveEx_enc(s1: state, d1: PageDb, s1':state, d1': PageDb,
+                                    s2: state, d2: PageDb, s2':state, d2': PageDb,
+                                    dispPg: PageNr, steps1:nat, steps2:nat,
+                                    obs: PageNr)
+    requires ValidState(s1) && ValidState(s2) &&
+             ValidState(s1') && ValidState(s2') &&
+             validPageDb(d1) && validPageDb(d2) && 
+             validPageDb(d1') && validPageDb(d2') && SaneConstants()
+    requires obs_entry(d1, d2, dispPg, obs)
+    requires validEnclaveExecution(s1, d1, s1', d1', dispPg, steps1)
+    requires validEnclaveExecution(s2, d2, s2', d2', dispPg, steps2);
+    requires loweq_pdb(d1, d2, obs)
+    requires s1.conf.nondet == s2.conf.nondet
+    requires OperandContents(s1, OLR) == OperandContents(s2, OLR)
+    requires user_regs(s1.regs) == user_regs(s2.regs)
+    requires mode_of_state(s1) != User && mode_of_state(s2) != User
+    requires !spsr_of_state(s1).f && !spsr_of_state(s1).i
+    requires !spsr_of_state(s2).f && !spsr_of_state(s2).i
+    requires spsr_same(s1, s2)
+    requires s1.conf.scr == s2.conf.scr;
+    ensures  obs_entry(d1', d2', dispPg, obs)
+    ensures  loweq_pdb(d1', d2', obs)
+    decreases steps1, steps2
+{
+    reveal validEnclaveExecution();
+
+    var retToEnclave1, s15, d15 := lemma_unpack_validEnclaveExecution(
+        s1, d1, s1', d1', dispPg, steps1);
+    var retToEnclave2, s25, d25 := lemma_unpack_validEnclaveExecution(
+        s2, d2, s2', d2', dispPg, steps2);
+
+    lemma_validEnclaveExecutionStep_validPageDb(s1, d1, s15, d15, dispPg, retToEnclave1);
+    lemma_validEnclaveExecutionStep_validPageDb(s2, d2, s25, d25, dispPg, retToEnclave2);
+    lemma_validEnclaveStep_enc(s1, d1, s15, d15, s2, d2, s25, d25,
+        dispPg, obs, retToEnclave1, retToEnclave2);
+
+    assert retToEnclave1 == retToEnclave2;
+
+    if(retToEnclave1) {
+        lemma_validEnclaveExecution(s15, d15, s1', d1', dispPg, steps1 - 1);
+        lemma_validEnclaveExecution(s25, d25, s2', d2', dispPg, steps2 - 1);
+        lemma_validEnclaveEx_enc(s15, d15, s1', d1', s25, d25, s2', d2',
+                                         dispPg, steps1 - 1, steps2 - 1, obs);
+        assert loweq_pdb(d1', d2', obs);
+    } else {
+        assert s2' == s25;
+        assert s1' == s15;
+        assert d1' == d15;
+        assert d2' == d25;
+        assert loweq_pdb(d1', d2', obs);
+    }
+
+}
+
+lemma lemma_validEnclaveStep_enc(s1: state, d1: PageDb, s1':state, d1': PageDb,
+                                      s2: state, d2: PageDb, s2':state, d2': PageDb,
+                                      dispPage:PageNr, obs: PageNr, ret1:bool, ret2:bool)
+    requires ValidState(s1) && ValidState(s2) &&
+             ValidState(s1') && ValidState(s2') &&
+             validPageDb(d1) && validPageDb(d2) && 
+             validPageDb(d1') && validPageDb(d2') && SaneConstants()
+    requires obs_entry(d1, d2, dispPage, obs)
+    requires validEnclaveExecutionStep(s1, d1, s1', d1', dispPage, ret1);
+    requires validEnclaveExecutionStep(s2, d2, s2', d2', dispPage, ret2);
+    requires loweq_pdb(d1, d2, obs)
+    requires s1.conf.nondet == s2.conf.nondet
+    requires OperandContents(s1, OLR) == OperandContents(s2, OLR)
+    requires user_regs(s1.regs) == user_regs(s2.regs)
+    requires mode_of_state(s1) != User && mode_of_state(s2) != User
+    requires spsr_same(s1, s2)
+    requires s1.conf.scr == s2.conf.scr;
+    ensures  obs_entry(d1', d2', dispPage, obs)
+    ensures  loweq_pdb(d1', d2', obs)
+    ensures  ret1 == ret2
+    ensures  ret1 ==> s1'.conf.scr == s2'.conf.scr;
+    ensures  ret1 ==> s1'.conf.nondet == s2'.conf.nondet
+    ensures  ret1 ==> OperandContents(s1', OLR) == OperandContents(s2', OLR)
+    ensures  ret1 ==> user_regs(s1'.regs) == user_regs(s2'.regs)
+{
+    reveal validEnclaveExecutionStep();
+    var s14, d14 :|
+        validEnclaveExecutionStep'(s1, d1, s14, d14, s1', d1',
+            dispPage, ret1);
+
+    var s24, d24 :|
+        validEnclaveExecutionStep'(s2, d2, s24, d24, s2', d2',
+            dispPage, ret2);
+    
+    lemma_updateUserPagesFromState_validPageDb(s14, d1, dispPage);
+    lemma_updateUserPagesFromState_validPageDb(s24, d2, dispPage);
+
+    assert validPageDb(d1);
+    assert validPageDb(d2);
+    assert validPageDb(d14);
+    assert validPageDb(d24);
+    assert validPageDb(d1');
+    assert validPageDb(d2');
+    lemma_validEnclaveStepPrime_enc(
+        s1, d1, s14, d14, s1', d1',
+        s2, d2, s24, d24, s2', d2',
+        dispPage, ret1, ret2, obs);
+}
+
+lemma lemma_userspaceExecutionFn_loweq_integ(
+s12: state, pc1:word, expc1:word, ex1:exception, s13:state,
+s22: state, pc2:word, expc2:word, ex2:exception, s23:state)
+    requires ValidState(s12) && ValidState(s13) && ValidState(s22) && 
+        ValidState(s23)
+    requires mode_of_state(s12) == User && mode_of_state(s22) == User
+    requires ExtractAbsPageTable(s12).Just? && ExtractAbsPageTable(s22).Just?
+    requires (s13, expc1, ex1) == userspaceExecutionFn(s12, pc1)
+    requires (s23, expc2, ex2) == userspaceExecutionFn(s22, pc2)
+    requires ExtractAbsPageTable(s12) == ExtractAbsPageTable(s22)
+    requires user_visible_state(s12, pc1, ExtractAbsPageTable(s12).v) ==
+        user_visible_state(s22, pc2, ExtractAbsPageTable(s22).v)
+    requires s12.conf.nondet == s22.conf.nondet
+    requires s12.conf.scr == s22.conf.scr
+    requires s12.conf.cpsr.f == s22.conf.cpsr.f;
+    requires s12.conf.cpsr.i == s22.conf.cpsr.i;
+    ensures  ex1 == ex2
+    ensures  user_regs(s13.regs) == user_regs(s23.regs)
+    ensures  expc1 == expc2
+    ensures  s13.conf.scr == s23.conf.scr
+    ensures s13.conf.nondet == s23.conf.nondet
+    ensures mode_of_exception(s13.conf, ex1) == mode_of_exception(s23.conf, ex2)
+    ensures cpsr in s13.sregs && cpsr in s23.sregs &&
+        s13.sregs[cpsr] == s23.sregs[cpsr]
+{
+    reveal userspaceExecutionFn();
+    assert user_regs(s13.regs) == user_regs(s23.regs) by {
+        var user_state1 := user_visible_state(s12, pc1, 
+            ExtractAbsPageTable(s12).v);
+        var user_state2 := user_visible_state(s22, pc2, 
+            ExtractAbsPageTable(s22).v);
+        var hr1 := havocUserRegs(s12.conf.nondet, user_state1, s12.regs);
+        var hr2 := havocUserRegs(s22.conf.nondet, user_state2, s22.regs);
+        assert s13.regs == hr1 by
+            { reveal userspaceExecutionFn(); }
+        assert s23.regs == hr2 by
+            { reveal userspaceExecutionFn(); }
+        assert user_state1 == user_state2;
+        assert s12.conf.nondet == s22.conf.nondet;
+        forall (r | r in USER_REGS() )
+            ensures hr1[r] ==
+                nondet_private_word(s12.conf.nondet, user_state1, NONDET_REG(r))
+            ensures hr2[r] ==
+                nondet_private_word(s22.conf.nondet, user_state2, NONDET_REG(r))
+            ensures hr1[r] == hr2[r]
+            ensures user_regs(hr1)[r] == user_regs(hr2)[r]
+        {
+        }
+        lemma_user_regs_domain(hr1, user_regs(hr1));
+        lemma_user_regs_domain(hr2, user_regs(hr2));
+        assert forall r :: r in user_regs(hr1) <==> r in user_regs(hr2);
+        assert forall r | r in user_regs(hr1) :: user_regs(hr1)[r] == user_regs(hr2)[r];
+    
+        eqregs(user_regs(hr1), user_regs(hr2));
+        assert user_regs(hr1) == user_regs(hr2);
+    }
+
+}
+
+lemma
+lemma_validEnclaveStepPrime_enc(
+s11: state, d11: PageDb, s14:state, d14:PageDb, r1:state, rd1:PageDb,
+s21: state, d21: PageDb, s24:state, d24:PageDb, r2:state, rd2:PageDb,
+dispPg:PageNr, retToEnclave1:bool, retToEnclave2:bool, obs: PageNr
+)
+    requires ValidState(s11) && ValidState(s21) &&
+             ValidState(r1)  && ValidState(r2)  &&
+             validPageDb(d11) &&
+             validPageDb(d21) && 
+             validPageDb(d14) && 
+             validPageDb(d24) && 
+             validPageDb(rd1) && 
+             validPageDb(rd2) && 
+             SaneConstants()
+    requires obs_entry(d11, d21, dispPg, obs)
+    requires validEnclaveExecutionStep'(s11,d11,s14,d14,r1,rd1,dispPg,retToEnclave1)
+    requires validEnclaveExecutionStep'(s21,d21,s24,d24,r2,rd2,dispPg,retToEnclave2)
+    requires OperandContents(s11, OLR) == OperandContents(s21, OLR)
+    requires user_regs(s11.regs) == user_regs(s21.regs)
+    requires loweq_pdb(d11, d21, obs)
+    requires s11.conf.nondet == s21.conf.nondet
+    requires mode_of_state(s11) != User && mode_of_state(s21) != User
+    requires spsr_same(s11, s21)
+    requires s11.conf.scr == s21.conf.scr;
+    ensures  obs_entry(rd1, rd2, dispPg, obs)
+    ensures  loweq_pdb(rd1, rd2, obs)
+    ensures  retToEnclave1 == retToEnclave2
+    ensures  retToEnclave1 ==> r1.conf.scr == r2.conf.scr
+    ensures  retToEnclave1 ==> r1.conf.nondet == r2.conf.nondet
+    ensures  retToEnclave1 ==> OperandContents(r1, OLR) == OperandContents(r2, OLR)
+    ensures  retToEnclave1 ==> user_regs(r1.regs) == user_regs(r2.regs)
+{                        
+    assert l1pOfDispatcher(d11, dispPg) == l1pOfDispatcher(d21, dispPg) by
+        { reveal loweq_pdb(); }
+    var l1p := l1pOfDispatcher(d11, dispPg);
+
+    assert dataPagesCorrespond(s11.m, d11);
+    assert dataPagesCorrespond(s21.m, d21);
+    
+    assert userspaceExecutionAndException(s11, s14);
+    assert userspaceExecutionAndException(s21, s24);
+
+    reveal userspaceExecutionAndException();
+
+    var s1', s12 :| userspaceExecutionAndException'(s11, s1', s12, s14);
+    var s2', s22 :| userspaceExecutionAndException'(s21, s2', s22, s24);
+
+    var pc1 := OperandContents(s11, OLR);
+    var pc2 := OperandContents(s21, OLR);
+    
+    var (s13, expc1, ex1) := userspaceExecutionFn(s12, pc1);
+    var (s23, expc2, ex2) := userspaceExecutionFn(s22, pc2);
+
+    // assert s12.m == s11.m;
+    // assert s22.m == s21.m;
+    assert cpsr_same(s12, s22) by {
+        lemma_eval_cpsrs(s11, s1', s12, s21, s2', s22);
+    }
+
+    assert pageTableCorresponds(s12, d11, l1p) &&
+        pageTableCorresponds(s22, d21, l1p) by
+    { 
+        assert pageTableCorresponds(s11, d11, l1p);
+        assert pageTableCorresponds(s21, d21, l1p);
+        reveal pageTableCorresponds();
+    }
+
+    var pt1 := ExtractAbsPageTable(s12);
+    var pt2 := ExtractAbsPageTable(s22);
+    assert pt1 == pt2 by {
+        lemma_eqpdb_pt_coresp(d11, d21, s12, s22, l1p, obs);
+    }
+    lemma_userStatesEquiv_atkr(
+        s11, s1', s12, s14, pc1, pt1, d11,
+        s21, s2', s22, s24, pc2, pt2, d21,
+        dispPg, obs, l1p);
+
+    lemma_userspaceExecutionFn_loweq_integ(
+        s12, pc1, expc1, ex1, s13,
+        s22, pc2, expc2, ex2, s23
+    );
+
+    var user_state1 := user_visible_state(s12, pc1, pt1.v);
+    var user_state2 := user_visible_state(s22, pc2, pt2.v);
+
+    assert s14.conf.ex == ex1 && s24.conf.ex == ex2;
+
+    assert s14.conf.nondet == s24.conf.nondet;
+
+    lemma_userspaceExec_atkr(
+        s11, s1', s12, s13, s14, d11, d14,
+        s21, s2', s22, s23, s24, d21, d24,
+        dispPg, obs, l1p);
+
+    assert user_regs(s14.regs) == user_regs(s13.regs)
+        && user_regs(s24.regs) == user_regs(s23.regs) by
+    {
+        lemma_exceptionTakenRegs(s13, ex1, expc1, s14);
+        lemma_exceptionTakenRegs(s23, ex2, expc2, s24);
+    }
+
+    assert OperandContents(s14, OLR) == OperandContents(s24, OLR) by
+    {
+        lemma_exceptionTakenRegs(s13, ex1, expc1, s14);
+        lemma_exceptionTakenRegs(s23, ex2, expc2, s24);
+        assert expc1 == expc2;
+    }
+
+    assert retToEnclave1 == retToEnclave2 by {
+        assert retToEnclave1 == isReturningSvc(s14);
+        assert retToEnclave2 == isReturningSvc(s24);
+        reveal ValidRegState();
+        assert s14.conf.ex == s24.conf.ex;
+        assert R0 in USER_REGS();
+        assert R0 in user_regs(s14.regs) && R0 in user_regs(s24.regs);
+        assert user_regs(s14.regs) == user_regs(s24.regs);
+        assert s14.regs[R0] == s24.regs[R0];
+
+    }
+
+    assert s14.conf.scr == s24.conf.scr;
+
+    var retToEnclave := retToEnclave1;
+
+    assert validDispatcherPage(d14, dispPg) && validDispatcherPage(d24, dispPg);
+
+    if(retToEnclave) {
+        var retRegs1 := svcHandled(s14, d14, dispPg).0;
+        var retRegs2 := svcHandled(s24, d24, dispPg).0;
+
+        lemma_svcHandled_validPageDb(s14, d14, dispPg, retRegs1, rd1);
+        lemma_svcHandled_validPageDb(s24, d24, dispPg, retRegs2, rd2);
+
+        lemma_svcHandled_loweq_pdb(s14, d14, rd1,
+            s24, d24, rd2, dispPg, obs);
+
+        assert r1.conf.nondet == r2.conf.nondet by {
+            assert s14.conf.nondet == s24.conf.nondet; 
+        }
+        assert loweq_pdb(rd1, rd2, obs);
+        assert r1.conf.nondet == r2.conf.nondet;
+        assert retRegs1 == retRegs2;
+        assert user_regs(r1.regs) == user_regs(r2.regs) by
+        { 
+            lemma_preEntryUserRegs(
+                s14, r1, retRegs1, rd1,
+                s24, r2, retRegs2, rd2, dispPg
+            );
+        }
+        assert OperandContents(r1, OLR) == OperandContents(r2, OLR);
+    } else {
+        assert validDispatcherPage(d14, dispPg) && validDispatcherPage(d24, dispPg);
+        lemma_exceptionTaken_atkr(
+            s13, s14, ex1, expc1, 
+            s23, s24, ex2, expc2);
+        lemma_exceptionHandled_atkr(s14, d14, rd1, s24, d24, rd2,
+             r1.regs[R0], r1.regs[R1], r2.regs[R0], r2.regs[R1],
+             dispPg, obs);
+
+        assert loweq_pdb(rd1, rd2, obs);
+    }
+}
+
+//-----------------------------------------------------------------------------
+// Resume
+//-----------------------------------------------------------------------------
+lemma lemma_resume_enc_ni(s1: state, d1: PageDb, s1':state, d1': PageDb,
+                               s2: state, d2: PageDb, s2':state, d2': PageDb,
+                               dispPage: word,
+                               obs: PageNr)
+    requires ni_reqs(s1, d1, s1', d1', s2, d2, s2', d2', obs)
+    requires smc_resume(s1, d1, s1', d1', dispPage)
+    requires smc_resume(s2, d2, s2', d2', dispPage)
+    requires loweq_pdb(d1, d2, obs)
+    requires s1.conf.nondet == s2.conf.nondet
+    ensures loweq_pdb(d1', d2', obs)
+{
+    reveal loweq_pdb();
+    var e1, e2 := smc_enter_err(d1, dispPage, true), smc_enter_err(d2, dispPage, true);
+    assert e1 == e2;
+
+    if(e1 == KOM_ERR_SUCCESS) {
+        var asp1, asp2 := d1[dispPage].addrspace, d2[dispPage].addrspace;
+        assert asp1 == asp2;
+        if(asp1 == obs) {
+            lemma_enter_enc_obs_enter(s1, d1, s1', d1',
+                                       s2, d2, s2', d2',
+                                       dispPage, 0, 0, 0, 
+                                       obs, true);
+        } else {
+            lemma_enter_loweq_pdb_not_obs(s1, d1, s1', d1',
+                                           s2, d2, s2', d2',
+                                           dispPage, 0, 0, 0,
+                                           asp1, obs, true);
+        }
+    } 
+}
